\documentclass[12pt]{article}

\usepackage[margin=1in]{geometry}
\usepackage{amsmath, amsthm, amssymb, amsfonts, mathrsfs, unicode-math}
\usepackage{esint}

\newcommand{\N}{\mathbb{N}}
\newcommand{\Z}{\mathbb{Z}}

\newenvironment{theorem}[2][Theorem]{\begin{trivlist}
\item[\hskip \labelsep {\bfseries #1}\hskip \labelsep {\bfseries #2.}]}{\end{trivlist}}
\newenvironment{lemma}[2][Lemma]{\begin{trivlist}
\item[\hskip \labelsep {\bfseries #1}\hskip \labelsep {\bfseries #2.}]}{\end{trivlist}}
\newenvironment{exercise}[2][Exercise]{\begin{trivlist}
\item[\hskip \labelsep {\bfseries #1}\hskip \labelsep {\bfseries #2.}]}{\end{trivlist}}
\newenvironment{problem}[2][Problem]{\begin{trivlist}
\item[\hskip \labelsep {\bfseries #1}\hskip \labelsep {\bfseries #2.}]}{\end{trivlist}}
\newenvironment{question}[2][Question]{\begin{trivlist}
\item[\hskip \labelsep {\bfseries #1}\hskip \labelsep {\bfseries #2.}]}{\end{trivlist}}
\newenvironment{corollary}[2][Corollary]{\begin{trivlist}
\item[\hskip \labelsep {\bfseries #1}\hskip \labelsep {\bfseries #2.}]}{\end{trivlist}}


\def\Xint#1{\mathchoice
{\XXint\displaystyle\textstyle{#1}}%
{\XXint\textstyle\scriptstyle{#1}}%
{\XXint\scriptstyle\scriptscriptstyle{#1}}%
{\XXint\scriptscriptstyle\scriptscriptstyle{#1}}%
\!\int}
\def\XXint#1#2#3{{\setbox0=\hbox{$#1{#2#3}{\int}$ }
\vcenter{\hbox{$#2#3$ }}\kern-.6\wd0}}
\def\ddashint{\Xint=}
\def\dashint{\Xint-}

% -----------------------------------------
% #########################################
% -----------------------------------------
% INTERMISSION
% -----------------------------------------
% #########################################
% -----------------------------------------

\begin{document}

\title{Harmonic Analysis}
\title{Homework #4}
\author{Dan Sokolsky}

\maketitle

\begin{exercise}{1}
\end{exercise}

\begin{proof}
  Let $\{Q_j\}$ be the cubes defined in the proof of the Calderón–Zygmund lemma. Let $S = \{x \in [0, 1)^n\ |\ M_4f(x) > \lambda\}$, where $x_0 = 0$ in the definition
  $$M_4f(x) = \sup_{Q \in \mathfrak{D}\ :\ Q \in [0, 1]^n} \dashint_Q |f|$$
  $(\subseteq)$ Let $Q_j = [a, b]^n$. Let $\tilde{Q}_j = [a, b)^n$. Then, $Q_j, \tilde{Q}_j$ only differ on a set of measure 0. By construction,
  $$\dashint_{\tilde{Q}_j} |f| = \dashint_{Q_j} |f| > \lambda$$
  so that $M_4f(x) > \lambda$ for all $x \in Q_j$. Therefore, $Q_j \subseteq S$ (for a.e. $x \in Q_j$). Thus, $\cup Q_j \subseteq S$ up to a set of measure 0.\\
  $(\supseteq)$ Let $x \in S$. Then there exists a dyadic cube $Q \subseteq [0, 1)^n$ such that
  $$\dashint_{Q} |f| > \lambda$$
  So that $Q = Q_j$ for some $j$. Thus $S \subseteq \cup Q_j$. Therefore, $S = \cup Q_j$ up to a set of measure 0.
\end{proof}

\begin{exercise}{2}
\end{exercise}

\begin{proof}
  $(a) (i)$ Since $\lambda > 0$ and $\mu\{|f| > \lambda\} \ge 0$, we have $\|f\|_{L^{p, \infty}}\ge 0$.\\
  $(ii)$
  $$\|kf\|_{L^{p, \infty}}^p = \sup_{\lambda > 0} \lambda^p \cdot \mu\{|kf| > \lambda\} = \sup_{\lambda > 0} \lambda^p \cdot \mu\{|f| > \frac{\lambda}{|k|}\} =$$
  $$\sup_{|k|\lambda > 0} (|k|\lambda)^p \cdot \mu\{|f| > \frac{|k|\lambda}{|k|}\} = \sup_{|k|\lambda > 0} (|k|\lambda)^p \cdot \mu\{|f| > \frac{|k|\lambda}{|k|}\} =
  |k|^p \cdot \sup_{|k|\lambda > 0} \lambda^p \cdot \mu\{|f| > \lambda\} =$$
  $$|k|^p \cdot \sup_{\lambda > 0} \lambda^p \cdot \mu\{|f| > \lambda\} = |k|^p \cdot \|f\|_{L^{p, \infty}}^p \iff \|kf\|_{L^{p, \infty}} = |k| \cdot \|f\|_{L^{p, \infty}}$$
  $(iii)$
  $$\|f + g\|_{L^{p, \infty}}^p = \sup_{\lambda > 0} \lambda^p \cdot \mu\{|f + g| > \lambda\} \le \sup_{\lambda > 0} \lambda^p \cdot (\mu\{|f| > \frac{\lambda}{2}\} + \mu\{|g| > \frac{\lambda}{2}\}) \le$$
  $$\sup_{\lambda > 0} \lambda^p \cdot (\mu\{|f| > \frac{\lambda}{2}\}) + \sup_{\lambda > 0} \lambda^p \cdot (\mu\{|g| > \lambda\}) =$$
  $$\sup_{2\lambda > 0} (2\lambda)^p \cdot (\mu\{|f| > \lambda\}) + \sup_{2\lambda > 0} (2\lambda)^p \cdot (\mu\{|g| > \lambda\}) =$$
  $$2^p\sup_{\lambda > 0} \lambda \cdot (\mu\{|f| > \lambda\}) + 2^p\sup_{\lambda > 0} \lambda \cdot (\mu\{|g| > \lambda\}) = 2^p (\|f\|_{L^{p, \infty}}^p + \|g\|_{L^{p, \infty}}^p)$$
  $$\iff \|f + g\|_{L^{p, \infty}} \le 2(\|f\|_{L^{p, \infty}} + \|g\|_{L^{p, \infty}})$$
  $(b)$
  $$\int_E |f| \ge \int_E \lambda = \lambda \mu(E)$$
  So that,
  $$\mu(E)^{\frac{1}{p}-1} \int_E |f| \ge \mu(E)^{\frac{1}{p}-1} \cdot \lambda \mu(E) = \lambda \cdot \mu(E)^{\frac{1}{p}}$$
  Thus,
  $$\|f\|' = \sup_{E: 0 < \mu(E) < \infty} \mu(E)^{\frac{1}{p}-1} \int_E |f| \ge \sup_{\lambda > 0} \lambda \mu\{|f| > \lambda\}^{\frac{1}{p}} = \|f\|_{L^{p, \infty}}$$
  $(c)$
  $$\int_E |f(x)| d\mu = \int_E \Big(\int_0^{|f(x)|} d\lambda \Big) du = \int_E \mu\{|f(x)| > \lambda\} d\lambda = \int_0^{\infty} \mu\{x \in E\ |\ |f(x)| > \lambda\} d\lambda \le$$
  $$\int_0^{\mu(E)^{-\frac{1}{p}}\|f\|_{L^{p, \infty}}} \mu(E) d\lambda + \int_{\mu(E)^{-\frac{1}{p}}\|f\|_{L^{p, \infty}}}^{\infty} \mu\{|f| > \lambda\} d\lambda \le$$
  $$\int_0^{\mu(E)^{-\frac{1}{p}}\|f\|_{L^{p, \infty}}} \mu(E) d\lambda + \int_{\mu(E)^{-\frac{1}{p}}\|f\|_{L^{p, \infty}}}^{\infty} \dfrac{\|f\|_{L^{p, \infty}}}{\lambda^p} d\lambda = $$
  $$\mu(E)^{-\frac{1}{p}}\|f\|_{L^{p, \infty}}\mu(E) + \|f\|_{L^{p, \infty}}^p \cdot \Big[\dfrac{\lambda^{1-p}}{1-p}\Big]_{\mu(E)^{-\frac{1}{p}}\|f\|_{L^{p, \infty}}}^{\infty} =$$
  $$\mu(E)^{\frac{p-1}{p}} \|f\|_{L^{p, \infty}} \cdot \dfrac{p}{p-1} \iff$$
  $$\mu(E)^{\frac{1}{p} - 1} \int_E |f| d\mu \le \dfrac{p}{p-1} \|f\|_{L^{p, \infty}}$$
  For all Borel sets $E$. Therefore,
  $$\|f\|' = \sup_{E: 0 < \mu(E) < \infty} \mu(E)^{\frac{1}{p} - 1} \int_E |f| d\mu \le \dfrac{p}{p-1} \|f\|_{L^{p, \infty}}$$
  $(d)$ We have
  $$\|f\|_{L^{p, \infty}} \le \|f\|' \le \dfrac{p}{p-1} \|f\|_{L^{p, \infty}}$$
  Thus the two norms are equivalent.
\end{proof}

\begin{exercise}{3}
\end{exercise}

\begin{proof}
  $(a)$ Let $R = |x - y|$. Since  $f \in \mathcal{S}(\mathbb{R}^n)$, $Df$ is bounded. Let $Df \le K$. Let us first estimate
  $$|\dashint_{B_R(x)} f - \dashint_{B_R(y)} f| = |\dashint_{B_R(x)} f(z + (y-x)) - f(z) dz| = |\dashint_{B_R(x)} \Big(\int_{z}^{z + (y - x)} Df(t) dt \Big) dz| \le$$
  $$\dashint_{B_R(x)} K \cdot |z + (y - x) - z| dz = \dashint_{B_R(x)} K \cdot |x - y| dz = K \cdot |x - y| \cdot \dfrac{1}{\mu(B_r(x))} \int_{B_r(x)} dz =$$
  $$K \cdot |x - y| \cdot 1 = K \cdot |x - y|$$
  Thus, by the lemma we proved in class, we have -
  $$|f(x) - f(x)| \le \Big|f(x) - \dashint_{B_R(x)} f\Big| + \Big|\dashint_{B_R(x)} f - \dashint_{B_R(y)} f\Big| + \Big|\dashint_{B_R(y)} f - f(y)\Big| \le$$
  $$C_1 \cdot |x-y| \cdot Mf(x) + K \cdot |x-y| + C_2 \cdot |x-y| \cdot Mf(y) \le$$
  $$C(Mf(x) + Mf(y)) \cdot |x-y|$$
  where $C = \max\{C_1, C_2, K\}$.\\\\
  $(b)$ By Hölder's inequality, we have, for all $s$,
  $$s \dashint_{B_s(x)} |Df| \le C(p, n) s^{1 - n + \frac{n}{p'}} \|Df\|_{L^p} = C(p, n) s^\alpha \|Df\|_{L^p}$$
  Thus
  $$s \cdot M(Df)(x) \le C(p, n) s^\alpha \|Df\|_{L^p}$$
  Substituting $s=\frac{r}{2},\frac{r}{4},\frac{r}{8}, \ldots$, we have
  $$r \cdot M(Df)(x) = \sum_{k=1}^{\infty} \frac{r}{2^k} \cdot M(Df)(x) \le \sum_{k=1}^{\infty} C(p, n) (\frac{r}{2^k})^\alpha \|Df\|_{L^p} \le$$ $$\sum_{k=1}^{\infty} C(p, n) r^\alpha \frac{1}{2^k} \|Df\|_{L^p} = C(p, n) r^\alpha \|Df\|_{L^p}$$

  Now, by the lemma we proved preceeding Sobolev's inequality, we have
  $$\Big|f(x) - \dashint_{B_R(x)} f\Big| \le C \cdot r \cdot M(Df)(x) \le C(p, n) r^\alpha \|Df\|_{L^p}$$
  $(c)$ Let $R=|x-y|$, as before. We had shown in $(b)$ that
  $$R \cdot M(Df)(x) \le C(p, n) R^\alpha \|Df\|_{L^p}$$
  It follows that
  $$M(Df)(x) \le C(p, n) R^{\alpha-1} \|Df\|_{L^p}$$
  Now from $(a)$,
  $$|f(x) - f(x)| \le C(Mf(x) + Mf(y)) \cdot |x-y| \le$$
  $$2 \cdot C(p, n) \cdot R^{\alpha-1} \cdot \|Df\|_{L^p} \cdot |x-y| = C(p, n) |x-y|^\alpha \|Df\|_{L^p}$$
\end{proof}

\end{document}
